lean/Lang/Basic.lean
@@ -1,1 +1,79 @@
-def hello := "world"
+import Lang.Ast
+import Mathlib.Data.List.AList
+import Mathlib.Data.Finset.Basic
+
+structure Loc where
+  loc : Nat
+deriving Repr, DecidableEq
+
+inductive Result {α β : Type} where
+  | ok (value : α)
+  | err (error : β)
+deriving Repr
+
+abbrev Env := @AList Name (fun _ => Loc)
+abbrev Memory := @AList Loc (fun _ => Bool)
+
+def typeCheckExpr (expr : Expr) (env : Env) : Bool := match expr with
+  | Expr.true => Bool.true
+  | Expr.false => Bool.true
+  | Expr.nand left right => (typeCheckExpr left env) && (typeCheckExpr right env)
+  | Expr.ident name => (AList.lookup name env).isSome
+  -- | Expr.ref of => Bool.true
+  -- | Expr.deref of => Bool.true
+
+theorem typeCheckExpr_nandLeft (h : typeCheckExpr (Expr.nand left right) env) : typeCheckExpr left env := by
+  unfold typeCheckExpr at h
+  simp [Bool.coe_and_iff] at h
+  apply And.left at h
+  exact h
+
+theorem typeCheckExpr_nandRight (h : typeCheckExpr (Expr.nand left right) env) : typeCheckExpr right env := by
+  unfold typeCheckExpr at h
+  simp [Bool.coe_and_iff] at h
+  apply And.right at h
+  exact h
+
+theorem typeCheckExpr_ident (h : typeCheckExpr (Expr.ident name) env) : (AList.lookup name env).isSome := by
+  unfold typeCheckExpr at h
+  exact h
+
+def evalExpr (expr : Expr) (env : Env) (mem : Memory) (h : typeCheckExpr expr env) : Bool := match expr with
+  | Expr.true => Bool.true
+  | Expr.false => Bool.false
+  | Expr.nand left right => !((evalExpr left env mem (typeCheckExpr_nandLeft h)) && (evalExpr right env mem (typeCheckExpr_nandRight h)))
+  | Expr.ident name => match AList.lookup name env, typeCheckExpr_ident h with
+    | some p, _ => true -- TODO: we need proofs about memory
+
+-- def evalStmt (expr : Expr) (env : Env) (mem : Memory) (h : typeCheckExpr expr env) : Bool := match expr with
+
+
+def typeCheckStmt (stmt : Stmt) (env : Env) : Bool := match stmt with
+  | Stmt.decl name value =>  (AList.lookup name env).isNone && (typeCheckExpr value env)
+  | Stmt.assign target value => (AList.lookup target env).isSome && (typeCheckExpr value env)
+  | Stmt.conditional condition body => (typeCheckExpr condition env) && (typeCheckStmt body env)
+
+def isClosedExpr (expr : Expr) (env : Env) : Bool := match expr with
+  | Expr.true => Bool.true
+  | Expr.false => Bool.true
+  | Expr.nand left right => (isClosedExpr left env) && (isClosedExpr right env)
+  | Expr.ident name => (AList.lookup name env).isSome
+
+theorem typeCheckExpr_isClosedExpr (expr : Expr) (h : (typeCheckExpr expr env) = true) : (isClosedExpr expr env) := match expr with
+  | Expr.true => by
+    apply h
+  | Expr.false => by
+    apply h
+  | Expr.nand left right => by
+    unfold typeCheckExpr at h
+    unfold isClosedExpr
+    simp [Bool.coe_and_iff] at h
+    simp [Bool.coe_and_iff]
+    have l := And.left h
+    have r := And.right h
+
+    have lp := by apply (typeCheckExpr_isClosedExpr left l)
+    have rp := by apply (typeCheckExpr_isClosedExpr right r)
+    exact ⟨lp, rp⟩
+  | Expr.ident name => by
+    apply h
